update

StructuredEncryption/src/Header.dfy
@@ -11,49 +11,70 @@ module TrussHeader {
   import Random
 
   type MessageID = x: seq<uint8> | |x| == 32 witness *
+  const UINT8_LIMIT := 256
+  type CMPEncryptedDataKey = x : CMP.EncryptedDataKey | ValidEncryptedDataKey(x) witness *
+  type CMPEncryptionContext  = x : CMP.EncryptionContext | ValidEncryptionContext(x) witness *
+  type CMPEncryptedDataKeyList = x : seq<CMPEncryptedDataKey> | |x| < UINT8_LIMIT
+  type Legend = x : seq<uint8> | |x| < UINT16_LIMIT
+  type CMPUtf8Bytes = x : CMP.Utf8Bytes | |x| < UINT16_LIMIT
+  
+  predicate method ValidEncryptionContext(x : CMP.EncryptionContext)
+  {
+    && |x| < UINT16_LIMIT
+    && (forall k <- x :: |k| < UINT16_LIMIT && |x[k]| < UINT16_LIMIT)
+  }
+
+  predicate method ValidEncryptedDataKey(x : CMP.EncryptedDataKey)
+  {
+    && |x.keyProviderId| < UINT16_LIMIT
+    && |x.keyProviderInfo| < UINT16_LIMIT
+    && |x.ciphertext| < UINT16_LIMIT
+  }
 
   datatype Header = Header (
     nameonly version : uint8,
     nameonly flavor : uint8,
     nameonly msgID : MessageID,
-    nameonly legend : seq<uint8>,
-    nameonly encContext : CMP.EncryptionContext,
-    nameonly dataKeys : CMP.EncryptedDataKeyList
+    nameonly legend : Legend,
+    nameonly encContext : CMPEncryptionContext,
+    nameonly dataKeys : CMPEncryptedDataKeyList
   )
   {
-    function method serialize() : (ret : Result<seq<uint8>, Error>)
-      ensures 
-       (&& SerializeLegend(legend).Success?
-        && SerializeContext(encContext).Success?
-        && SerializeDataKeys(dataKeys).Success?) ==> ret.Success?
-
-      ensures ret.Success? ==>
-        && |ret.value| > 66
-        && ret.value[|ret.value|-32..] == HmacSha384(ret.value[..|ret.value|-32], EncodeAscii("TRUSS_COMMIT_KEY"))
-        && SerializeLegend(legend).Success?
-        && SerializeContext(encContext).Success?
-        && SerializeDataKeys(dataKeys).Success?
-        && ret.value == (
+    // Header to Bytes
+    function method {:opaque} serialize() : (ret : seq<uint8>)
+      ensures
+        && |ret| > 66
+        //= specification/structured-encryption/header.md#header-commitment
+        //= type=implication
+        //# The Header Commitment MUST be calculated as a 256-bit HmacSha384,
+        //# with all preceding header bytes as the message
+        //# and a commitment key of "TRUSS_COMMIT_KEY"
+        && ret[|ret|-32..] == HmacSha384(ret[..|ret|-32], EncodeAscii("TRUSS_COMMIT_KEY"))
+        //= specification/structured-encryption/header.md#header-format
+        //= type=implication
+        //# The serialized form of the header MUST be
+        // | Length (bytes) | Meaning |
+        // |---|---|
+        // | 1 | Format Version |
+        // | 1 | Format Flavor |
+        // | 32 | Message ID|
+        // | Variable | Encrypt Legend |
+        // | Variable | Encrypt Context|
+        // | Variable | Encrypted Data Keys |
+        // | 32 | Header Commitment |
+        && ret == (
             [version]
           + [flavor]
           + msgID
-          + SerializeLegend(legend).value
-          + SerializeContext(encContext).value
-          + SerializeDataKeys(dataKeys).value
-          + HmacSha384(ret.value[..|ret.value|-32], EncodeAscii("TRUSS_COMMIT_KEY"))
+          + SerializeLegend(legend)
+          + SerializeContext(encContext)
+          + SerializeDataKeys(dataKeys)
+          + HmacSha384(ret[..|ret|-32], EncodeAscii("TRUSS_COMMIT_KEY"))
         )
-      ensures ret.Success? ==>
-        && GetLegend(ret.value[34..]).Success?
-        //&& var leg := GetLegend(ret.value[34..]).value; GetContext(ret.value[34+leg.1..]).Success?
-        /*
-              && var leg := GetLegend(data[34..]).value; GetContext(data[34+leg.1..]).Success?
-      && var cont := GetContext(data[34+leg.1..]).value; GetDataKeys(data[34+leg.1+cont.1..]).Success?
-      && var dk := GetDataKeys(data[34+leg.1+cont.1..]).value; |data| == 34+leg.1+cont.1+dk.1+32) ==>
-*/
     {
-      var context :- SerializeContext(encContext);
-      var keys :- SerializeDataKeys(dataKeys);
-      var leg :- SerializeLegend(legend);
+      var context := SerializeContext(encContext);
+      var keys := SerializeDataKeys(dataKeys);
+      var leg := SerializeLegend(legend);
       var baseHeader :=
           [version]
         + [flavor]
@@ -63,10 +84,11 @@ module TrussHeader {
         + keys
       ;
       var commitment := HmacSha384(baseHeader, EncodeAscii("TRUSS_COMMIT_KEY"));
-       Success(baseHeader + commitment)
+      baseHeader + commitment
     }
   }
 
+  // config to Header
   function method Create(
       schema : CryptoSchema,
       msgID : MessageID,
@@ -74,7 +96,33 @@ module TrussHeader {
       dataKeys : CMP.EncryptedDataKeyList
     )
     : (ret : Result<Header, Error>)
+    ensures ret.Success? ==>
+      //= specification/structured-encryption/header.md#format-version
+      //= type=implication
+      //# The Version MUST be `0x01`.
+      && ret.value.version == 1
+      //= specification/structured-encryption/header.md#format-flavor
+      //= type=implication
+      //# The flavor MUST be one of these two values.
+      // | Value | Meaning |
+      // |---|---|
+      // | 0x01 | Signatures enabled (default) |
+      // | 0x00 | Signatures disabled |
+      && ret.value.flavor == 1
+      //= specification/structured-encryption/header.md#key-value-pair-count
+      //= type=implication
+      //# The value of this field MUST be greater than 0.
+      && 0 < |encContext|
+      //= specification/structured-encryption/header.md#encrypted-data-key-count
+      //= type=implication
+      //# This value MUST be greater than 0.
+      && 0 < |dataKeys|
   {
+    :- Need(0 < |encContext|, E("Encryption context must not be empty"));
+    :- Need(ValidEncryptionContext(encContext), E("Invalid Encryption Context"));
+    :- Need(0 < |dataKeys|, E("There must be at least one data key"));
+    :- Need(|dataKeys| < UINT8_LIMIT, E("Too many data keys."));
+    :- Need(forall x | x in dataKeys :: ValidEncryptedDataKey(x), E("Invalid Data Key"));
     var legend :- MakeLegend(schema);
     Success(Header(
       version := 1,
@@ -86,6 +134,7 @@ module TrussHeader {
     ))
   }
   
+  // bytes to Header
   function method Deserialize(data : seq<uint8>)
     : (ret : Result<Header, Error>)
     ensures
@@ -99,24 +148,18 @@ module TrussHeader {
       && var dk := GetDataKeys(data[34+leg.1+cont.1..]).value;
       && |data| == 34+leg.1+cont.1+dk.1+32) <==>
       ret.Success?
-/*
     ensures ret.Success? ==> 
-      && |data| > 66
-      && data[|data|-32..] == HmacSha384(data[..|data|-32], EncodeAscii("TRUSS_COMMIT_KEY"))
-      && SerializeLegend(ret.value.legend).Success?
-      && SerializeContext(ret.value.encContext).Success?
-      && SerializeDataKeys(ret.value.dataKeys).Success?
       && var v := ret.value;
-        data == (
-            [v.version]
-          + [v.flavor]
-          + v.msgID
-          + SerializeLegend(v.legend).value
-          + SerializeContext(v.encContext).value
-          + SerializeDataKeys(v.dataKeys).value
-          + HmacSha384(data[..|data|-32], EncodeAscii("TRUSS_COMMIT_KEY"))
-        )
-        */
+      && v.version == data[0]
+      && v.flavor == data[1]
+      && v.msgID == data[2..34]
+      && var data1 := data[34..];
+      && GetLegend(data1).Success?
+      && var legendAndLen := GetLegend(data1).value;
+      && v.legend == legendAndLen.0
+      && var data2 := data1[legendAndLen.1..];
+      && var contextAndLen := GetContext(data2).value;
+      && v.encContext == contextAndLen.0
   {
     :- Need(|data| > 66, E("Serialized header too short."));
     var storedCommitment := data[|data|-32..];
@@ -127,7 +170,6 @@ module TrussHeader {
     var msgID := data[2..34];
     var data1 := data[34..];
 
-    // legend needs schema
     var legendAndLen :- GetLegend(data1);
     var legend := legendAndLen.0;
     var data2 := data1[legendAndLen.1..];
@@ -150,80 +192,211 @@ module TrussHeader {
       dataKeys := dataKeys
     ))
   }
-/*
-    lemma RoundTrip2(h : seq<uint8>)
-      requires Deserialize(h).Success?
-      ensures Deserialize(h).value.serialize().Success?
-      ensures h == Deserialize(h).value.serialize().value
-    {
-    }
-    */
-/*
-    lemma RoundTrip(h : Header)
-      requires h.serialize().Success?
-      ensures deserialize(h.serialize().value).Success?
-      ensures h == deserialize(h.serialize().value).value
-    {
-      assert deserialize(h.serialize().value).Success?;
-      RoundTrip2(h.serialize().value);
-      var n := deserialize(h.serialize().value).value;
-      LegendRoundTrip(h.legend);
-      DataKeysRoundTrip(h.dataKeys);
-      ContextRoundTrip(h.encContext);
-      assert h.version == n.version;
-      assert h.flavor == n.flavor;
-      assert h.msgID == n.msgID;
-      assert h.legend == n.legend;
-      assert h.encContext == n.encContext;
-      assert h.dataKeys == n.dataKeys;
-    }
-  */
 
+  function method HmacSha384(data : seq<uint8>, key : seq<uint8>) : (ret : seq<uint8>)
+    ensures |ret| == 32
+  {
+    [0,0,0,0,0,0,0,0,0,0,0,0,0,0,0,0,0,0,0,0,0,0,0,0,0,0,0,0,0,0,0,0]
+  }
+
+  predicate method ByteLess(x : uint8, y : uint8)
+  {
+    x < y
+  }
+
+  predicate method CharLess(x : char, y : char)
+  {
+    x < y
+  }
+
+  function method ToUInt16(x : nat)
+    : (ret : Result<uint16, Error>)
+    ensures x < UINT16_LIMIT ==> ret.Success?
+  {
+    :- Need(x < UINT16_LIMIT, E("Value too big for 16 bits"));
+    Success(x as uint16)
+  }
+
+  // string to Error
   function method E(s : string) : Error {
     StructuredEncryptionException(message := s)
   }
-  function method MakeLegend(schema : CryptoSchema) : Result<seq<uint8>, Error>
+
+  // CryptoSchema to Bytes
+  function method MakeLegend(schema : CryptoSchema)
+    : (ret : Result<Legend, Error>)
+    ensures ret.Success? ==>
+      && schema.content.SchemaMap?
+      && AllActions(schema.content.SchemaMap)
+      //= specification/structured-encryption/header.md#encrypt-legend-bytes
+      //= type=implication
+      //# The length of this serialized value (in bytes) MUST equal the number of authenticated fields indicated
+      //# by the caller's [Authenticate Schema](./structures.md#authenticate-schema).
+      && |ret.value| == CountAuthAttrs(schema.content.SchemaMap)
+      && var attrs := ComputeSetToOrderedSequence2(schema.content.SchemaMap.Keys, CharLess);
+      && MakeLegend2(attrs, schema.content.SchemaMap).Success?
+      && ret.value == MakeLegend2(attrs, schema.content.SchemaMap).value
+
   {
     :- Need(schema.content.SchemaMap?, E("Should be a SchemaMap"));
+    :- Need(AllActions(schema.content.SchemaMap), E("All members of SchemaMap must be Actions"));
+    //= specification/structured-encryption/header.md#encrypt-legend-bytes
+    //# The Encrypt Legend Bytes MUST be serialized as follows:
+    // 1. Order every authenticated attribute in the item lexicographically by the attribute name.
+    // 2. For each authenticated attribute, in order,
+    // append one of the byte values specified above to indicate whether
+    // that field should be encrypted.
     var attrs := ComputeSetToOrderedSequence2(schema.content.SchemaMap.Keys, CharLess);
     MakeLegend2(attrs, schema.content.SchemaMap)
   }
 
+  function method MakeOneLegend(x : CryptoAction)
+    : (ret : seq<uint8>)
+    //= specification/structured-encryption/header.md#encrypt-legend-bytes
+    //= type=implication
+    //# Each Crypto Action MUST be encoded as follows
+    // | Field | Length (bytes) | Interpreted as |
+    // | ----- | -------------- | -------------- |
+    // | Encrypt Legend Length | 2 | big endian UInt16 |
+    // | Encrypt Legend Bytes | Variable. Equal to the value specified in the previous 2 bytes (Encrypt Legend Length). | Bytes |
+    // - `0x65` (`e` in UTF-8, for "Encrypt and Sign") means that a particular field was encrypted
+    //   and included in the signature calculation.
+    //   This indicates that this field MUST be attempted to be decrypted during decryption.
+    // - `0x73` (`s` in UTF-8, for "Sign Only") means that a particular field was not encrypted,
+    //   but still included in the signature calculation.
+    //   This indicates that this field MUST NOT be attempted to be decrypted during decryption.
+    // - no entry if the attribute is not signed
+    ensures match (x) {
+      case ENCRYPT_AND_SIGN => ret == [0x65]
+      case SIGN_ONLY => ret == [0x73]
+      case DO_NOTHING => ret == []
+    }
+  {
+    match (x) {
+      case ENCRYPT_AND_SIGN => [0x65]
+      case SIGN_ONLY => [0x73]
+      case DO_NOTHING => []
+    }
+  }
 
+  function method IsAuthAttr(x : CryptoAction) : nat
+  {
+    match (x) {
+      case ENCRYPT_AND_SIGN => 1
+      case SIGN_ONLY => 1
+      case DO_NOTHING => 0
+    }
+  }
 
-  function method MakeLegend2(attrs : seq<string>, data : CryptoSchemaMap, acc : seq<uint8> := [])
-    : Result<seq<uint8>, Error>
+  function method {:tailrecursion} AllActions2(attrs : seq<string>, data : CryptoSchemaMap) : (ret : bool)
     requires forall k <- attrs :: k in data
+    ensures ret ==> (forall k <- attrs :: data[k].content.Action?)
   {
     if |attrs| == 0 then
-      Success(acc)
+      true
+    else if !data[attrs[0]].content.Action? then
+      false
     else
-      :- Need(data[attrs[0]].content.Action?, E("Must be map of actions"));
-      var legendChar := match data[attrs[0]].content.Action {
-        case ENCRYPT_AND_SIGN => [0x65]
-        case SIGN_ONLY => [0x73]
-        case DO_NOTHING => []
-      };
-      MakeLegend2(attrs[1..], data, acc + legendChar)
+      AllActions2(attrs[1..], data)
+  }
+
+  function method AllActions(data : CryptoSchemaMap) : (ret : bool)
+    ensures ret ==> (forall v <- data.Values :: v.content.Action?)
+  {
+    var attrs := ComputeSetToOrderedSequence2(data.Keys, CharLess);
+    AllActions2(attrs, data)
+  }
+
+  function method CountAuthAttrs2(attrs : seq<string>, data : CryptoSchemaMap)
+    : (ret : nat)
+    requires forall k <- attrs :: k in data
+    requires forall x | x in attrs :: data[x].content.Action?
+    ensures |attrs| > 0 ==> ret == CountAuthAttrs2(attrs[1..], data) + IsAuthAttr(data[attrs[0]].content.Action)
+  {
+    if |attrs| == 0 then
+      0
+    else 
+      CountAuthAttrs2(attrs[1..], data) + IsAuthAttr(data[attrs[0]].content.Action)
+  }
+
+  function method CountAuthAttrs(data : CryptoSchemaMap)
+    : nat
+    requires forall x <- data.Values :: x.content.Action?
+  {
+    var attrs := ComputeSetToOrderedSequence2(data.Keys, CharLess);
+    CountAuthAttrs2(attrs, data)
+  }
+
+  function method {:tailrecursion} MakeLegend2(
+      attrs : seq<string>,
+      data : CryptoSchemaMap,
+      serialized : Legend := []
+    )
+    : (ret : Result<Legend, Error>)
+    requires AllActions(data)
+    requires forall k <- attrs :: k in data
+    requires CountAuthAttrs2(attrs, data) + |serialized| == CountAuthAttrs(data)
+    ensures ret.Success? ==>
+      && |ret.value| == CountAuthAttrs(data)
+  {
+    if |attrs| == 0 then
+      Success(serialized)
+    else
+      if (|serialized| + 1) >= UINT16_LIMIT then
+        Failure(E("Legend Too Long."))
+      else
+        var legendChar := MakeOneLegend(data[attrs[0]].content.Action);
+        MakeLegend2(attrs[1..], data, serialized + legendChar)
+  }
+
+  function method {:opaque} SerializeLegend(x : Legend)
+    : (ret : seq<uint8>)
+    //= specification/structured-encryption/header.md#encrypt-legend
+    //= type=implication
+    //# The Encrypt Legend MUST be serialized as
+    ensures
+      && |ret| == 2 + |x|
+      && SeqToUInt16(ret[0..2]) == |x| as uint16
+      && ret[2..] == x
+
+  {
+    UInt16ToSeq(|x| as uint16) + x
+  }
+
+  function method GetLegend(data : seq<uint8>)
+    : (ret : Result<(Legend, nat), Error>)
+    ensures ret.Success? ==>
+      && ret.value.1 <= |data|
+      && ret.value.1 == |ret.value.0| + 2
+      && ret.value.0 == data[2..ret.value.1]
+  {
+    :- Need(2 <= |data|, E("Invalid Header"));
+    var len := SeqToUInt16(data[0..2]);
+    var size := len as nat + 2;
+    :- Need(size <= |data|, E("Invalid header"));
+    Success((data[2..size], size))
   }
 
   function method GetContext(data : seq<uint8>)
-    : (ret : Result<(CMP.EncryptionContext, nat), Error>)
+    : (ret : Result<(CMPEncryptionContext, nat), Error>)
     ensures ret.Success? ==>
       && ret.value.1 <= |data|
-      //&& SerializeContext(ret.value.0).Success?
+    ensures (
+      && 2 <= |data|
+      && GetContext2(SeqToUInt16(data[0..2]) as nat, data, data[2..], (map[], 2)).Success?
+    ) ==> ret.Success?
+
   {
     :- Need(2 <= |data|, E("Invalid Header"));
-    var count := SeqToUInt16(data[0..2]);
+    var count := SeqToUInt16(data[0..2]) as nat;
     GetContext2(count, data, data[2..], (map[], 2))
   }
 
   function method GetOneContext(data : seq<uint8>)
-    : (ret : Result<(CMP.Utf8Bytes,CMP.Utf8Bytes,nat), Error>)
+    : (ret : Result<(CMPUtf8Bytes, CMPUtf8Bytes, nat), Error>)
     ensures ret.Success? ==>
       && ret.value.2 <= |data|
-      && SerializeOneContext(ret.value.0, ret.value.1).Success?
-      && SerializeOneContext(ret.value.0, ret.value.1).value == data[..ret.value.2]
+      && SerializeOneContext(ret.value.0, ret.value.1) == data[..ret.value.2]
     ensures (
       && 2 <= |data|
       && var keylen := SeqToUInt16(data[0..2]) as nat;
@@ -232,7 +405,7 @@ module TrussHeader {
       && var valueLen := SeqToUInt16(data[keylen+2..keylen+4]) as nat;
       && keylen + valueLen + 4 <= |data|
       && ValidUTF8Seq(data[keylen+4..keylen + valueLen + 4])
-    ) <==> ret.Success? && SerializeOneContext(ret.value.0, ret.value.1).value == data[..ret.value.2]
+    ) <==> ret.Success? && SerializeOneContext(ret.value.0, ret.value.1) == data[..ret.value.2]
   {
     :- Need(2 <= |data|, E("Invalid Header"));
     var keylen := SeqToUInt16(data[0..2]) as nat;
@@ -246,127 +419,228 @@ module TrussHeader {
     :- Need(ValidUTF8Seq(value), E("Invalid Header"));
     Success((key, value, kvLen))
   }
-  function method {:tailrecursion} GetContext2(count : uint16, origData : seq<uint8>, data : seq<uint8>, acc : (CMP.EncryptionContext, nat))
-    : (ret : Result<(CMP.EncryptionContext, nat), Error>)
-    requires acc.1 <= |origData|
-    requires acc.1 + |data| == |origData|
+  function method {:tailrecursion} GetContext2(count : nat, origData : seq<uint8>, data : seq<uint8>, deserialized : (CMPEncryptionContext, nat))
+    : (ret : Result<(CMPEncryptionContext, nat), Error>)
+    requires deserialized.1 <= |origData|
+    requires deserialized.1 + |data| == |origData|
+    requires data == origData[deserialized.1..]
     ensures ret.Success? ==> 
       && ret.value.1 <= |origData|
+      && (count > 0 ==> GetOneContext(data).Success?)
   {
     if count == 0 then
-      Success(acc)
+      Success(deserialized)
     else
-      var kv :- GetOneContext(data);
-      GetContext2(count-1, origData, data[2+|kv.0|+2+|kv.1|..], (acc.0[kv.0 := kv.1], acc.1 + kv.2))
+      if |deserialized.0| + 1 >= UINT16_LIMIT then
+        Failure(E("Too much context"))
+      else
+        var kv :- GetOneContext(data);
+        GetContext2(count-1, origData, data[2+|kv.0|+2+|kv.1|..], (deserialized.0[kv.0 := kv.1], deserialized.1 + kv.2))
   }
 
-  function method HmacSha384(data : seq<uint8>, key : seq<uint8>) : (ret : seq<uint8>)
-    ensures |ret| == 32
+  //= specification/structured-encryption/header.md#key-value-pair-entries
+  //= type=implication
+  //# This sequence MUST NOT contain duplicate entries.
+  // true because CMPEncryptionContext is a map
+  function method {:opaque} SerializeContext(x : CMPEncryptionContext)
+    : (ret : seq<uint8>)
+    ensures
+      && |ret| >= 2
+      //= specification/structured-encryption/header.md#key-value-pair-entries
+      //= type=implication
+      //# These entries MUST have entries sorted, by key,
+      //# in ascending order according to the UTF-8 encoded binary value.
+      && var keys := ComputeSetToOrderedSequence2(x.Keys, ByteLess);
+      //= specification/structured-encryption/header.md#encrypt-context
+      //= type=implication
+      //# The Encryption Context MUST be serialized as follows
+      // | Field | Length (bytes) | Interpreted as |
+      // | ----- | -------------- | -------------- |
+      // | Key Value Pair Count | 2 | big endian UInt16 |
+      // | Key Value Pair Entries | Variable. Determined by the count and length of each key-value pair. | Key Value Pair Entries |
+      && ret == UInt16ToSeq(|x| as uint16) + SerializeContext2(keys, x)
   {
-    [0,0,0,0,0,0,0,0,0,0,0,0,0,0,0,0,0,0,0,0,0,0,0,0,0,0,0,0,0,0,0,0]
+    var keys := ComputeSetToOrderedSequence2(x.Keys, ByteLess);
+    UInt16ToSeq(|x| as uint16) + SerializeContext2(keys, x)
   }
 
-  predicate method ByteLess(x : uint8, y : uint8)
+  function method SerializeOneContext(key : CMPUtf8Bytes, value : CMPUtf8Bytes)
+    : (ret : seq<uint8>)
+    //= specification/structured-encryption/header.md#key-value-pair-entries
+    //= type=implication
+    //# Each Key Value Pair MUST be serialized as follows
+    // | Field | Length (bytes) | Interpreted as |
+    // | ----- | -------------- | -------------- |
+    // | Key Length | 2 | big endian UInt16 |
+    // | Key | Variable. Equal to the value specified in the previous 2 bytes (Key Length). | UTF-8 encoded bytes |
+    // | Value Length | 2 | big endian UInt16 |
+    // | Value | Variable. Equal to the value specified in the previous 2 bytes (Value Length). | UTF-8 encoded bytes |
+    ensures ret == UInt16ToSeq(|key| as uint16) + key + UInt16ToSeq(|value| as uint16) + value
   {
-    x < y
-  }
-  predicate method CharLess(x : char, y : char)
-  {
-    x < y
-  }
-
-  function method ToUInt16(x : nat)
-    : (ret : Result<uint16, Error>)
-    ensures x < UINT16_LIMIT ==> ret.Success?
-  {
-    :- Need(x < UINT16_LIMIT, E("Value too big for 16 bits"));
-    Success(x as uint16)
-  }
-  function method {:opaque} SerializeLegend(x : seq<uint8>)
-    : (ret : Result<seq<uint8>, Error>)
-    ensures |x| < UINT16_LIMIT <==> ret.Success?
-    ensures ret.Success? ==>
-      && |ret.value| == 2 + |x|
-      && SeqToUInt16(ret.value[0..2]) == |x| as uint16
-      && ret.value[2..] == x
-  {
-    var legSize :- ToUInt16(|x|);
-    Success(UInt16ToSeq(legSize) + x)
+    UInt16ToSeq(|key| as uint16) + key + UInt16ToSeq(|value| as uint16) + value
   }
 
-  function method GetLegend(data : seq<uint8>)
-    : (ret : Result<(seq<uint8>, nat), Error>)
+  function method SerializeOneDataKey(k : CMPEncryptedDataKey)
+    : (ret : seq<uint8>)
+    //= specification/structured-encryption/header.md#encrypted-data-key-entries
+    //= type=implication
+    //# Each Encrypted Data Key MUST be serialized as follows
+    // | Field | Length (bytes) | Interpreted as |
+    // | ----- | -------------- | -------------- |
+    // | Key Provider ID Length  | 2 | big endian UInt16 |
+    // | Key Provider ID | Variable. Equal to the value specified in the previous 2 bytes (Key Provider ID Length). | UTF-8 encoded bytes |
+    // | Key Provider Information Length | 2 | big endian UInt16 |
+    // | Key Provider Information | Variable. Equal to the value specified in the previous 2 bytes (Key Provider Information Length). | Bytes |
+    // | Encrypted Data Key Length | 2 | big endian UInt16 |
+    // | Encrypted Data Key | Variable. Equal to the value specified in the previous 2 bytes (Encrypted Data Key Length). | Bytes |
+    ensures
+      && var provIdSize := ToUInt16(|k.keyProviderId|).value;
+      && var provInfoSize := ToUInt16(|k.keyProviderInfo|).value;
+      && var cipherSize := ToUInt16(|k.ciphertext|).value;
+      && ret == (
+          UInt16ToSeq(provIdSize)
+        + k.keyProviderId
+        + UInt16ToSeq(provInfoSize)
+        + k.keyProviderInfo
+        + UInt16ToSeq(cipherSize)
+        + k.ciphertext
+      )
+  {
+      UInt16ToSeq(|k.keyProviderId| as uint16)
+    + k.keyProviderId
+    + UInt16ToSeq(|k.keyProviderInfo| as uint16)
+    + k.keyProviderInfo
+    + UInt16ToSeq(|k.ciphertext| as uint16)
+    + k.ciphertext
+  }
+  
+
+  function method GetOneDataKey(data : seq<uint8>)
+    : (ret : Result<(CMPEncryptedDataKey, nat), Error>)
     ensures ret.Success? ==>
       && ret.value.1 <= |data|
-      && ret.value.1 == |ret.value.0| + 2
-      && ret.value.0 == data[2..ret.value.1]
-      && SerializeLegend(ret.value.0).Success?
+      && |SerializeOneDataKey(ret.value.0)| == ret.value.1
+      && SerializeOneDataKey(ret.value.0) == data[0..ret.value.1]
   {
     :- Need(2 <= |data|, E("Invalid Header"));
-    var len := SeqToUInt16(data[0..2]);
-    var size := len as nat + 2;
-    :- Need(size <= |data|, E("Invalid header"));
-    Success((data[2..size], size))
+    var provIdSize := SeqToUInt16(data[0..2]) as nat;
+    :- Need(provIdSize + 2 < |data|, E("Invalid Header"));
+    var provId := data[2..2+provIdSize];
+    :- Need(ValidUTF8Seq(provId), E("Invalid Header"));
+    var part1Size := 2 + provIdSize;
+
+    :- Need(part1Size+2 <= |data|, E("Invalid Header"));
+    var provInfoSize := SeqToUInt16(data[part1Size..part1Size+2]) as nat;
+    :- Need(part1Size + provInfoSize + 2 < |data|, E("Invalid Header"));
+    var provInfo := data[part1Size+2..part1Size+2+provInfoSize];
+    var part2Size := part1Size + 2 + provInfoSize;
+
+    :- Need(part2Size+2 <= |data|, E("Invalid Header"));
+    var cipherSize := SeqToUInt16(data[part2Size..part2Size+2]) as nat;
+    :- Need(part2Size + cipherSize + 2 <= |data|, E("Invalid Header"));
+    var cipher := data[part2Size+2..part2Size+2+cipherSize];
+    var part3Size := part2Size + 2 + cipherSize;
+
+    var edk := CMP.EncryptedDataKey(keyProviderId := provId, keyProviderInfo := provInfo, ciphertext := cipher);
+    Success((edk, part3Size))
   }
 
-  lemma LegendRoundTrip(x : seq<uint8>)
-    requires |x| < UINT16_LIMIT
-    ensures SerializeLegend(x).Success?
-    ensures GetLegend(SerializeLegend(x).value).Success?
-    ensures var ret := GetLegend(SerializeLegend(x).value).value;
+  function method {:tailrecursion} SerializeContext2(keys : seq<CMPUtf8Bytes>, x : CMPEncryptionContext)
+    : (ret : seq<uint8>)
+    requires forall k <- keys :: k in x
+  {
+    if |keys| == 0 then
+      []
+    else
+      SerializeOneContext(keys[0], x[keys[0]]) + SerializeContext2(keys[1..], x)
+  }
+
+  function method SerializeDataKeys(x : CMPEncryptedDataKeyList)
+    : (ret : seq<uint8>)
+      //= specification/structured-encryption/header.md#encrypted-data-keys
+      //= type=implication
+      //# The Encrypted Data Keys MUST be serialized as follows
+      // | Field | Length (bytes) | Interpreted as |
+      // | ----- | -------------- | -------------- |
+      // | Encrypted Data Key Count | 1 | big endian UInt16 |
+      // | [Encrypted Data Key Entries | Variable. Determined by the count and length of each key-value pair. | Encrypted Data Key Entries |
+      ensures
+        && 1 <= |ret|
+        && ret[0] as nat == |x|
+        && ret == [|x| as uint8] + SerializeDataKeys2(x)
+  {
+    var body := SerializeDataKeys2(x);
+    [|x| as uint8] + body
+  }
+
+  function method {:tailrecursion} SerializeDataKeys2(x : CMPEncryptedDataKeyList)
+    : (ret : seq<uint8>)
+  {
+    if |x| == 0 then
+      []
+    else
+      SerializeOneDataKey(x[0]) + SerializeDataKeys2(x[1..])
+  }
+
+  function method GetDataKeys(data : seq<uint8>)
+    : (ret : Result<(CMPEncryptedDataKeyList, nat), Error>)
+    ensures ret.Success? ==>
+      && ret.value.1 <= |data|
+      && 1 <= |data|
+      && 1 <= ret.value.1
+      && |ret.value.0| == data[0] as nat
+      && GetDataKeys2(|ret.value.0|, |ret.value.0|, data, data[1..], ([], 1)).Success?
+  {
+    :- Need(1 <= |data|, E("Invalid Header"));
+    var count := data[0] as nat;
+    GetDataKeys2(count, count, data, data[1..], ([], 1))
+  }
+
+  function method {:tailrecursion} GetDataKeys2(count : nat, origCount : nat, origData : seq<uint8>, data : seq<uint8>, deserialized : (CMPEncryptedDataKeyList, nat))
+    : (ret : Result<(CMPEncryptedDataKeyList, nat), Error>)
+    requires deserialized.1 <= |origData|
+    requires deserialized.1 + |data| == |origData|
+    requires origCount == count + |deserialized.0|
+    ensures ret.Success? ==>
+      && ret.value.1 <= |origData|
+      && ret.value.1 >= deserialized.1
+      && (count > 0 ==> GetOneDataKey(data).Success?)
+      && |ret.value.0| == origCount
+
+  {
+    if count == 0 then
+      Success(deserialized)
+    else
+      if |deserialized.0| >= 255 then
+        Failure(E("Too Many Data Keys"))
+      else
+        var edk :- GetOneDataKey(data);
+        assert SerializeOneDataKey(edk.0) == data[..edk.1];
+        GetDataKeys2(count-1, origCount, origData, data[edk.1..], (deserialized.0 + [edk.0], deserialized.1+edk.1)) 
+  }
+
+// End code, begin proofs
+
+  lemma SerializeLegendRoundTrip(x : Legend)
+    ensures GetLegend(SerializeLegend(x)).Success?
+    ensures var ret := GetLegend(SerializeLegend(x)).value;
       && ret.0 == x
       && ret.1 == |x| + 2
-      && ret.1 == |SerializeLegend(x).value|
+      && ret.1 == |SerializeLegend(x)|
   {}
 
-  function method {:opaque} SerializeContext(x : CMP.EncryptionContext)
-    : (ret : Result<seq<uint8>, Error>)
-    ensures ret.Success? ==>
-      && |ret.value| >= 2
-      && var keys := ComputeSetToOrderedSequence2(x.Keys, ByteLess); SerializeContext2(keys, x).Success?
+  lemma GetLegendRoundTrip(x : seq<uint8>)
+    requires GetLegend(x).Success?
+    ensures
+      && var ret := SerializeLegend(GetLegend(x).value.0);
+      && ret == x[..GetLegend(x).value.1]
   {
-    var mapSize :- ToUInt16(|x|);
-    var keys := ComputeSetToOrderedSequence2(x.Keys, ByteLess);
-    var body :- SerializeContext2(keys, x);
-    Success(UInt16ToSeq(mapSize) + body)
   }
 
-  function GOC(key : CMP.Utf8Bytes, value : CMP.Utf8Bytes) : (ret : bool)
-    requires SerializeOneContext(key, value).Success?
-    ensures ret == true
+  lemma SerializeOneContextRoundTrip(key : CMPUtf8Bytes, value : CMPUtf8Bytes)
+    ensures GetOneContext(SerializeOneContext(key, value)).Success?
   {
-    SerializeOneContextRoundTrip(key, value);
-    assert GetOneContext(SerializeOneContext(key, value).value).Success?;
-    GetOneContext(SerializeOneContext(key, value).value).Success?
-  }
-/*
-  lemma SerializeContextRoundTrip(x : CMP.EncryptionContext)
-    requires SerializeContext(x).Success?
-    {
-      var keys := ComputeSetToOrderedSequence2(x.Keys, ByteLess);
-      assert SerializeContext2(keys, x).Success?;
-      assert forall k <- keys :: SerializeOneContext(k, x[k]).Success?;
-      //assert forall k <- keys :: GetOneContext(SerializeOneContext(k, x[k]).value).Success?;
-      assert forall k <- keys :: GOC(k, x[k]);
-      assert GetContext(SerializeContext(x).value).Success?;
-      //&& GetContext(SerializeContext(x).value).value.0 == x
-
-    }
-*/
-  function method SerializeOneContext(key : CMP.Utf8Bytes, value : CMP.Utf8Bytes)
-    : (ret : Result<seq<uint8>, Error>)
-    //ensures ret.Success? ==> GetOneContext(ret.value).Success? -- must be a lemma or circular dependency
-  {
-    var keySize :- ToUInt16(|key|);
-    var valSize :- ToUInt16(|value|);
-    Success(UInt16ToSeq(keySize) + key + UInt16ToSeq(valSize) + value)
-  }
-
-  lemma SerializeOneContextRoundTrip(key : CMP.Utf8Bytes, value : CMP.Utf8Bytes)
-    requires SerializeOneContext(key, value).Success?
-    ensures GetOneContext(SerializeOneContext(key, value).value).Success?
-  {
-    var data := SerializeOneContext(key, value).value;
+    var data := SerializeOneContext(key, value);
     assert 2 <= |data|;
     var keylen := SeqToUInt16(data[0..2]) as nat;
     assert keylen + 4 <= |data|;
@@ -377,118 +651,243 @@ module TrussHeader {
     assert data[keylen+4..keylen + valueLen + 4] == value;
     assert ValidUTF8Seq(data[keylen+4..keylen + valueLen + 4]);
   }
-  function method {:tailrecursion} SerializeContext2(keys : seq<CMP.Utf8Bytes>, x : CMP.EncryptionContext, acc : seq<uint8> := [])
-    : (ret : Result<seq<uint8>, Error>)
-    requires forall k <- keys :: k in x
-    ensures ret.Success? ==>
-      && forall k <- keys :: SerializeOneContext(k, x[k]).Success?
-  {
-    if |keys| == 0 then
-      Success(acc)
-    else
-      var kv :- SerializeOneContext(keys[0], x[keys[0]]);
-      SerializeOneContextRoundTrip(keys[0], x[keys[0]]);
-      SerializeContext2(keys[1..], x, acc + kv)
-  }
-
-  function method SerializeDataKeys(x : CMP.EncryptedDataKeyList)
-    : Result<seq<uint8>, Error>
-  {
-    var listSize :- ToUInt16(|x|);
-    var body :- SerializeDataKeys2(x);
-    Success(UInt16ToSeq(listSize) + body)
-  }
-  function method SerializeOneDataKey(k : CMP.EncryptedDataKey)
-    : (ret : Result<seq<uint8>, Error>)
-    //ensures ret.Success? ==> GetOneDataKey(ret.value).Success?
-  {
-    var provIdSize :- ToUInt16(|k.keyProviderId|);
-    var provInfoSize :- ToUInt16(|k.keyProviderInfo|);
-    var cipherSize :- ToUInt16(|k.ciphertext|);
-      Success(
-        UInt16ToSeq(provIdSize)
-      + k.keyProviderId
-      + UInt16ToSeq(provInfoSize)
-      + k.keyProviderInfo
-      + UInt16ToSeq(cipherSize)
-      + k.ciphertext)
-  }
-  function method {:tailrecursion} SerializeDataKeys2(x : CMP.EncryptedDataKeyList, acc : seq<uint8> := [])
-    : Result<seq<uint8>, Error>
-  {
-    if |x| == 0 then
-      Success(acc)
-    else
-      var k :- SerializeOneDataKey(x[0]);
-      SerializeDataKeys2(x[1..], acc + k)
-  }
-
-  function method GetDataKeys(data : seq<uint8>)
-    : (ret : Result<(CMP.EncryptedDataKeyList, nat), Error>)
-    ensures ret.Success? ==>
-      && ret.value.1 <= |data|
-      // && SerializeDataKeys(ret.value.0).Success?
-  {
-    :- Need(2 <= |data|, E("Invalid Header"));
-    var count := SeqToUInt16(data[0..2]);
-    GetDataKeys2(count, data, data[2..], ([], 2))
-  }
-  function method GetOneDataKey(data : seq<uint8>)
-    : (ret : Result<(CMP.EncryptedDataKey, nat), Error>)
-    ensures ret.Success? ==> SerializeOneDataKey(ret.value.0).Success?
-  {
-    :- Need(2 <= |data|, E("Invalid Header"));
-    var provIdSize := SeqToUInt16(data[0..2]) as nat;
-    :- Need(provIdSize + 4 < |data|, E("Invalid Header"));
-    var provId := data[2..2+provIdSize];
-    :- Need(ValidUTF8Seq(provId), E("Invalid Header"));
-    var part1Size := 2 + provIdSize;
-
-    :- Need(part1Size+2 <= |data|, E("Invalid Header"));
-    var provInfoSize := SeqToUInt16(data[part1Size..part1Size+2]) as nat;
-    :- Need(part1Size + provInfoSize + 4 < |data|, E("Invalid Header"));
-    var provInfo := data[part1Size+2..part1Size+2+provInfoSize];
-    var part2Size := part1Size + 2 + provInfoSize;
-
-    :- Need(part2Size+2 <= |data|, E("Invalid Header"));
-    var cipherSize := SeqToUInt16(data[part2Size..part2Size+2]) as nat;
-    :- Need(part2Size + cipherSize + 2 < |data|, E("Invalid Header"));
-    var cipher := data[part2Size+2..part2Size+2+cipherSize];
-    var part3Size := part2Size + 2 + cipherSize;
-
-    var edk := CMP.EncryptedDataKey(keyProviderId := provId, keyProviderInfo := provInfo, ciphertext := cipher);
-    Success((edk, part3Size))
-  }
-  function method {:tailrecursion} GetDataKeys2(count : uint16, origData : seq<uint8>, data : seq<uint8>, acc : (CMP.EncryptedDataKeyList, nat))
-    : (ret : Result<(CMP.EncryptedDataKeyList, nat), Error>)
-    requires acc.1 <= |origData|
-    requires acc.1 + |data| == |origData|
-    ensures ret.Success? ==>
-      && ret.value.1 <= |origData|
-      && (count > 0 ==> GetOneDataKey(data).Success?)
-  {
-    if count == 0 then
-      Success(acc)
-    else
-      var edk :- GetOneDataKey(data);
-      GetDataKeys2(count-1, origData, data[edk.1..], (acc.0 + [edk.0], acc.1+edk.1)) 
-  }
-/*
-  lemma DataKeysRoundTrip(x : CMP.EncryptedDataKeyList)
-    requires SerializeDataKeys(x).Success?
-    ensures GetDataKeys(SerializeDataKeys(x).value).Success?
-    ensures GetDataKeys(SerializeDataKeys(x).value).value.0 == x  
-    ensures GetDataKeys(SerializeDataKeys(x).value).value.1 == |SerializeDataKeys(x).value|
   
-  lemma ContextRoundTrip(x : CMP.EncryptionContext)
-    requires SerializeContext(x).Success?
-    ensures GetContext(SerializeContext(x).value).Success?
-    ensures GetContext(SerializeContext(x).value).value.0 == x  
-    ensures GetContext(SerializeContext(x).value).value.1 == |SerializeContext(x).value|
+  lemma GetOneContextRoundTrip(data : seq<uint8>)
+    requires GetOneContext(data).Success?
+    ensures
+      && var cont := GetOneContext(data).value;
+      && SerializeOneContext(cont.0, cont.1) == data[..cont.2]
+  {}
+
+  lemma SerializeOneDataKeyRoundTrip(k : CMPEncryptedDataKey)
+    ensures
+      && var data := SerializeOneDataKey(k);
+      && GetOneDataKey(data).Success?
+      && GetOneDataKey(data).value.0 == k
+      && GetOneDataKey(data).value.1 == |data|
+    {
+      var data := SerializeOneDataKey(k);
+      assert 2 <= |data|;
+      var provIdSize := SeqToUInt16(data[0..2]) as nat;
+      assert provIdSize + 2 < |data|;
+      var provId := data[2..2+provIdSize];
+      assert provId == k.keyProviderId;
+    }
+
+  lemma GetOneDataKeyRoundTrip(data : seq<uint8>)
+    requires GetOneDataKey(data).Success?
+    ensures
+      && var cont := GetOneDataKey(data).value;
+      && SerializeOneDataKey(cont.0) == data[..cont.1]
+  {}
+
+  lemma GetDataKeysRoundTrip(data : seq<uint8>)
+    requires GetDataKeys(data).Success?
+    ensures
+      && var dk := GetDataKeys(data).value;
+      && SerializeDataKeys(dk.0) == data[..dk.1]
+  {
+    var dk := GetDataKeys(data).value;
+    GetDataKeys2RoundTrip(data, |dk.0|);
+    assert SerializeDataKeys(dk.0) == [|dk.0| as uint8] + SerializeDataKeys2(dk.0);
+  }
+
+  // Yes, four axioms, I am deeply ashamed, but I think the associated proofs still have value
+
+  lemma {:axiom} GetDataKeys2RoundTrip(data : seq<uint8>, count : nat)
+    requires 1 <= |data|
+    requires GetDataKeys2(count, count, data, data[1..], ([], 1)).Success?
+    ensures
+      && var dk := GetDataKeys2(count, count, data, data[1..], ([], 1)).value;
+      && SerializeDataKeys2(dk.0) == data[1..dk.1]    
+
+  lemma {:axiom} SerializeDataKeys2RoundTrip(data : CMPEncryptedDataKeyList)
+    ensures
+      && var bytes := SerializeDataKeys2(data);
+      && var count := |data|;
+      && var bytes2 := [count as uint8] + bytes;
+      && GetDataKeys2(count, count, bytes2, bytes2[1..], ([], 1)).Success?
+      && GetDataKeys2(count, count, bytes2, bytes2[1..], ([], 1)).value.0 == data
+      && GetDataKeys2(count, count, bytes2, bytes2[1..], ([], 1)).value.1 == |bytes2|
+
+  lemma {:axiom} SerializeContextRoundTrip(x : CMPEncryptionContext)
+    ensures GetContext(SerializeContext(x)).Success?
+    ensures GetContext(SerializeContext(x)).value.0 == x  
+    ensures GetContext(SerializeContext(x)).value.1 == |SerializeContext(x)|
   
-  lemma ContextRoundTrip2(x : seq<uint8>)
+  lemma {:axiom} GetContextRoundTrip(x : seq<uint8>)
     requires GetContext(x).Success?
-    ensures SerializeContext(GetContext(x).value.0).Success?
-    ensures SerializeContext(GetContext(x).value.0).value == x
-    */
+    ensures SerializeContext(GetContext(x).value.0) == x
+  
+  lemma GetOneContextExt(x : seq<uint8>, y : seq<uint8>)
+    requires x <= y
+    requires GetOneContext(x).Success?
+    ensures
+      && GetOneContext(y).Success?
+      && GetOneContext(x).value == GetOneContext(y).value
+    {
+      assert 2 <= |y|;
+      var keylen := SeqToUInt16(y[0..2]) as nat;
+      assert(keylen + 4 <= |y|);
+      var key := y[2..keylen+2];
+      assert x[2..keylen+2] == y[2..keylen+2];
+      assert(ValidUTF8Seq(key));
+      var valuelen := SeqToUInt16(y[keylen+2..keylen+4]) as nat;
+      var kvLen := 2 + keylen + 2 + valuelen;
+      assert kvLen <= |y|;
+      var value := y[keylen+4..kvLen];
+      assert x[keylen+4..kvLen] == y[keylen+4..kvLen];
+      assert ValidUTF8Seq(value);
+    }
+
+  lemma GetContext2Ext2(count : nat, origX : seq<uint8>, origY : seq<uint8>, x : seq<uint8>, y : seq<uint8>, deserialized : (CMPEncryptionContext, nat))
+    requires x <= y
+    requires origX <= origY
+    requires deserialized.1 <= |origX|
+    requires deserialized.1 <= |origY|
+    requires deserialized.1 + |x| == |origX|
+    requires deserialized.1 + |y| == |origY|
+    requires x == origX[deserialized.1..]
+    requires y == origY[deserialized.1..]
+    requires GetContext2(count, origX, x, deserialized).Success?
+    requires count == 0 ||  |deserialized.0| + 1 < UINT16_LIMIT
+    ensures
+        && GetContext2(count, origY, y, deserialized).Success?
+        && GetContext2(count, origX, x, deserialized).value == GetContext2(count, origY, y, deserialized).value
+  {
+    if count == 0 {
+    } else {
+      assert |deserialized.0| + 1 < UINT16_LIMIT;
+      assert GetOneContext(x).Success?;
+      GetOneContextExt(x, y);
+      assert GetOneContext(y).Success?;
+      var kv := GetOneContext(y).value;
+      var kvLen := 2+|kv.0|+2+|kv.1|;
+      assert x[kvLen..] <= y[kvLen..];
+      GetContext2Ext2(count-1, origX, origY, x[kvLen..],  y[kvLen..], (deserialized.0[kv.0 := kv.1], deserialized.1 + kv.2));
+    }
+  }
+
+  lemma GetContext2Ext(count : nat, x : seq<uint8>, y : seq<uint8>)
+    requires 2 <= |x|
+    requires x <= y
+    requires GetContext2(count, x, x[2..], (map[], 2)).Success?
+    ensures
+        && GetContext2(count, y, y[2..], (map[], 2)).Success?
+        && GetContext2(count, x, x[2..], (map[], 2)).value == GetContext2(count, y, y[2..], (map[], 2)).value
+  {
+    GetContext2Ext2(count, x, y, x[2..], y[2..], (map[], 2));
+  }
+
+  lemma SerializeDataKeysRoundTrip(data : CMPEncryptedDataKeyList)
+    ensures
+      && var bytes := SerializeDataKeys(data);
+      && GetDataKeys(bytes).Success?
+      && GetDataKeys(bytes).value.0 == data
+      && GetDataKeys(bytes).value.1 == |bytes|
+  {
+    SerializeDataKeys2RoundTrip(data);
+  }
+
+  lemma GetContextExt2(x : seq<uint8>, y : seq<uint8>)
+    requires 2 <= |x|
+    requires x <= y
+    ensures GetContext(x).Success? ==>
+      && GetContext(y).Success?
+      && GetContext(x).value == GetContext(y).value
+  {
+    if GetContext(x).Success? {
+      var countX := SeqToUInt16(x[0..2]) as nat;
+      var countY := SeqToUInt16(y[0..2]) as nat;
+      assert countX == countY;
+      assert GetContext2(countX, x, x[2..], (map[], 2)).Success?;
+      GetContext2Ext(countX, x, y);
+    }
+  }
+  lemma GetContextExt()
+    ensures forall x : seq<uint8>, y : seq<uint8> | 2 <= |x|  && x <= y ::
+      GetContext(x).Success? ==>
+        && GetContext(y).Success?
+        && GetContext(x).value == GetContext(y).value
+    {
+      forall x : seq<uint8>, y : seq<uint8> | 2 <= |x|  && x <= y ensures
+        GetContext(x).Success? ==>
+          && GetContext(y).Success?
+          && GetContext(x).value == GetContext(y).value {
+            GetContextExt2(x, y);
+          }
+    }
+
+  lemma DeserializeRoundTrip(data : seq<uint8>)
+    requires Deserialize(data).Success?
+    ensures
+      && var ret := Deserialize(data).value;
+      && |data| > 66
+      && data[|data|-32..] == HmacSha384(data[..|data|-32], EncodeAscii("TRUSS_COMMIT_KEY"))
+      && data == (
+            [ret.version]
+          + [ret.flavor]
+          + ret.msgID
+          + SerializeLegend(ret.legend)
+          + SerializeContext(ret.encContext)
+          + SerializeDataKeys(ret.dataKeys)
+          + HmacSha384(data[..|data|-32], EncodeAscii("TRUSS_COMMIT_KEY"))
+        )
+    {
+      var ret := Deserialize(data).value;
+      assert |data| > 66;
+      assert data[|data|-32..] == HmacSha384(data[..|data|-32], EncodeAscii("TRUSS_COMMIT_KEY"));
+      var leg := SerializeLegend(ret.legend);
+      GetLegendRoundTrip(leg);
+      var data1 := data[34..];
+      assert GetLegend(data1).Success?;
+      var legendAndLen := GetLegend(data1).value;
+      var data2 := data1[legendAndLen.1..];
+      var contextAndLen := GetContext(data2).value;
+      GetContextRoundTrip(data2);
+      SerializeContextRoundTrip(ret.encContext);
+      SerializeDataKeysRoundTrip(ret.dataKeys);
+      var cont := SerializeContext(ret.encContext);
+      GetDataKeysRoundTrip(cont);
+    }
+
+
+    lemma SerializeRoundTrip(h : Header)
+      ensures Deserialize(h.serialize()).Success?
+      ensures h == Deserialize(h.serialize()).value
+    {
+      var data := h.serialize();
+
+      SerializeLegendRoundTrip(h.legend);
+      SerializeContextRoundTrip(h.encContext);
+      SerializeDataKeysRoundTrip(h.dataKeys);
+
+      assert GetLegend(SerializeLegend(h.legend)).Success?;
+      assert GetContext(SerializeContext(h.encContext)).Success?;
+      assert GetDataKeys(SerializeDataKeys(h.dataKeys)).Success?;
+
+      var data1 := data[34..];
+
+      var serLegend1 := SerializeLegend(h.legend);
+      var serLegend2 := data1[..|serLegend1|];
+      assert serLegend1 == serLegend2;
+      var legendAndLenR := GetLegend(serLegend2);
+      assert legendAndLenR.Success?;
+      GetLegendRoundTrip(data1);
+      var legendAndLen := legendAndLenR.value;
+      var legend := legendAndLen.0;
+      var data2 := data1[legendAndLen.1..];
+
+      var serContext1 := SerializeContext(h.encContext);
+      var serContext2 := data2[..|serContext1|];
+      assert serContext1 == serContext2;
+      var contextAndLenR := GetContext(serContext2);
+      assert contextAndLenR.Success?;
+      var contextAndLen := contextAndLenR.value;
+      GetContextRoundTrip(serContext2);
+      GetContextExt();
+      GetContextRoundTrip(data2);
+      var encContext := contextAndLen.0;
+      var data3 := data2[contextAndLen.1..];
+    }
 }
